dijkstra/dijkstra_spec1.v
@@ -2,7 +2,9 @@ Require Import CertiGraph.graph.SpaceAdjMatGraph1.
 Require Import CertiGraph.dijkstra.dijkstra_env.
 
 (* A separate file with the underlying PQ spec-ed out *)
-Require Export CertiGraph.priq.priq_arr_specs.
+(* Require Export CertiGraph.priq.priq_arr_specs. (* *) *)
+Require Export CertiGraph.binheap.verif_binary_heap_pro. 
+
 
 (* Dijkstra-specific imports *)
 Require Import CertiGraph.dijkstra.MathDijkGraph.
@@ -83,14 +85,23 @@ Section DijkstraSpec.
           data_at Tsh (tarray tint size) (map Vint (map Int.repr dist)) (pointer_val_val dist_ptr)).
 
   Definition Gprog : funspecs :=
-    ltac:(with_library prog
-                       [(@init_spec size _);
-                       (@push_spec size inf _);
-                       (@pq_emp_spec size inf _);
-                       (@adjustWeight_spec size inf _);
-                       (@popMin_spec size inf Z_EqDec _);
-                       freePQ_spec;
+    ltac:(with_library prog [
+                         (* (@init_spec size _); *)
+                       (* (@push_spec size inf _); *)
+                       (* (@pq_emp_spec size inf _); *)
+                       (* (@adjustWeight_spec size inf _); *)
+                       (* (@popMin_spec size inf Z_EqDec _); *)
+                       (* freePQ_spec; *)
                        getCell_spec;
-                       dijkstra_spec]).
+                       dijkstra_spec;
+                       
+                       remove_min_nc_spec;
+                       pq_insert_nc_spec; 
+                       pq_size_spec;
+                       pq_make_spec;
+                       pq_edit_priority_spec;
+                       pq_free_spec]).
+
+
 
 End DijkstraSpec.
